test-suite/TestFun.v
@@ -1,13 +1,12 @@
 (* -*- coq-prog-args : ("-debug" "-type-in-type") -*-  *)
 
-(* (* Is is necessary to import Template.trad for the definition of prod' *) *)
-(* Require Import Template.Translation Template.trad. *)
+Require Import Template.Translation Template.sigma.
+Open Scope sigma_scope.
 
-(* Let T := Type. *)
-(* Check (T : T). *)
+Let T := Type.
+Check (T : T).
 
-(* Translate prod'. *)
-(* Translate pair'. *)
+(* Translate pair. *)
 (* (* Translate fst'. *) *)
 (* (* Translate snd'. *) *)
 (* Translate bool. *)
@@ -16,44 +15,40 @@
 
 (* Definition n : (fun x => x) Type := nat. *)
 
-(* Definition g := prod Prop Type. *)
-(* Definition f := g. *)
+Definition g := prod Prop Type.
+Definition f := g.
 
-(* Axiom tr : nat. *)
+Axiom tr : nat.
 
-(* (* Fail Translate tr. *) *)
-(* Translate g. *)
-(* Translate f. *)
-(* Print fᵗ. *)
+Fail Translate tr.
+Translate g.
+Translate f.
+Print fᵗ.
 
-(* Implement t2 : bool as totot. *)
-(* econstructor. *)
-(* Defined. *)
-(* Print t2. *)
-(* Print totot. *)
+Implement t2 : bool as totot.
+econstructor.
+Defined.
+Print t2.
+Print totot.
 
-(* Definition t4 := (t2, true). *)
-(* Translate t4. *)
+Definition t4 := (t2, true).
+Translate t4.
 
-(* Implement t3 : t2 = t2. *)
-(* econstructor. *)
-(* Defined. *)
+Implement t3 : t2 = t2.
+econstructor.
+Defined.
 
-(* Definition t3' := pair' _ _ t3 nat. *)
-(* Translate t3'. *)
-(* Print t3'ᵗ. *)
+Definition t3' := pair t3 nat.
+Translate t3'.
+Print t3'ᵗ.
 
-(* Implement nnnn : (nat -> nat). *)
-(* (* Implement nnnn : prod' (nat -> nat) bool. *) *)
-(* econstructor; econstructor. *)
-(* Defined. *)
+Implement nnnn : (nat -> nat).
+econstructor; econstructor.
+Defined.
 
-(* Set Printing Universes. *)
-
-(* Definition t5 := forall X:Set, X. *)
-(* (* Print Sorted Universes. *) *)
-(* Translate t5. *)
-(* Print Sorted Universes. *)
+Definition t5 := forall X:Set, X.
+Translate t5.
+Print t5ᵗ.
 
 (* (* Axiom a : forall X, X. *) *)
 
@@ -86,27 +81,27 @@
 (* (* Open Scope my_scope. *) *)
 
 
-(* Tactic Notation "intro'" ident(X) := econstructor; [intro X|exact true]. *)
-(* Tactic Notation "intros'" := repeat (refine (_, true); intro). *)
-(* Tactic Notation "specialize'" hyp(H) uconstr(t) := apply fst' in H; specialize (H t). *)
+Tactic Notation "intro'" ident(X) := econstructor; [intro X|exact true].
+Tactic Notation "intros'" := repeat (refine (mk_sig _ true); intro).
+Tactic Notation "specialize'" hyp(H) uconstr(t) := apply π1 in H; specialize (H t).
 
 (* Translate False. *)
 (* Translate eq. *)
 
 (* (* This translation allow to implement the negation of funext. *) *)
 (* (* Test Quote  *) *)
-(* Implement notFunext : *)
-(*   ((forall (A B : Set) (f g : A -> B), (forall x:A, f x = f x) -> f = g) -> False). *)
-(* Proof. *)
-(*   intro' H. *)
-(*   specialize' H unit. *)
-(*   specialize' H unit. *)
-(*   specialize' H (pair' _ _ (fun x => x) true). *)
-(*   specialize' H (pair' _ _ (fun x => x) false). cbn in *. *)
-(*   specialize' H (pair' _ _ (fun x => eq_refl) true). *)
-(*   apply (f_equal snd') in H; cbn in H. *)
-(*   discriminate H. *)
-(* Defined. *)
+Implement notFunext :
+  ((forall (A B : Set) (f g : A -> B), (forall x:A, f x = f x) -> f = g) -> False).
+Proof.
+  intro' H.
+  specialize' H unit.
+  specialize' H unit.
+  specialize' H (fun x => x; true).
+  specialize' H (fun x => x; false). cbn in *.
+  specialize' H (fun x => eq_refl; true).
+  apply (f_equal (@π2 _ (fun _ => bool))) in H; cbn in H.
+  discriminate H.
+Defined.
 
 (* (* (* A more constructive version on inhabited types. *) *) *)
 (* (* Implement notFunext' : forall (A B : Type), *) *)
@@ -145,230 +140,6 @@
 
 (* (* ** Some check of the translation on other types. *** *) *)
 
-(* Implement f : forall (f : Type -> Type), f Type. *)
-(* Abort. *)
-
-(* Implement foo : forall A B : Type, forall (f g : A -> B), forall x, f x = g x. *)
-(* Abort. *)
-
-(* Implement wqd : forall (A : Type) (B : A -> Prop), forall x, B x. *)
-(* Abort. *)
-
-(* Implement foo : forall (A : Type) (a : A) (p : a = a), p = eq_refl a. *)
-(* Abort. *)
-
-
-(* Is is necessary to import Template.trad for the definition of prod' *)
-Require Import Template.Translation Template.trad.
-
-(* Test Quote Type. *)
-(* Set Printing Universes. *)
-(* Make Definition t := (Ast.tSort (Ast.sType BinNums.xH)). *)
-(* Print t. *)
-(* Print Universes. *)
-
-Let T := Type.
-Check (T : T).
-
-
-Open Scope sigma_scope.
-
-Implement t' : Set.
-cbn. exists nat. exact (fun _ => bool).
-Defined.
-
-Definition t := Set.
-Translate t.
-Fail Implement Existing t.
-Print Visibility.
-
-Implement y : Type.
-refine (@mk_sig Type (fun A : Type => A -> Type) Type _).
-auto.
-Defined.
-
-Fail Translate unit.
-Implement Existing unit.
-exact (mk_sig unit (fun _ => unit)).
-Defined.
-Print unitᵗ.
-
-Implement Existing tt.
-unshelve econstructor. exact tt. exact tt.
-Defined.
-
-Fail Translate tt.
-
-Implement ttt : unit.
-cbn.
-econstructor.
-exact tt. exact tt.
-Defined.
-Print tttᵗ.
-
-Axiom tr : unit.
-Fail Translate tr.
-Implement Existing tr.
-Admitted.
-
-
-Notation "'TYPE'" := (exists A, A -> Type).
-Notation "'El' A" := (sigma (π1 A) (π2 A)) (at level 20).
-
-Definition Type_cst := Type.
-Translate Type_cst as Typeᶠ.
-
-(* Definition Typeᶠ : El Typeᶠ := *)
-(*   @mk_sig Type (fun A => A -> Type) Type (fun A => A -> Type). *)
-
-Check Typeᶠ : El Typeᶠ.
-
-Definition mkTYPE (A₀ : Type) (Aᴿ : A₀ -> Type) : El Typeᶠ :=
-  @mk_sig Type (fun A₀ => A₀ -> Type) A₀ Aᴿ.
-
-Definition Prodᶠ (A : El Typeᶠ) (B : El A -> El Typeᶠ) : El Typeᶠ :=
-  mkTYPE
-    (forall x : El A, (B x).1)
-    (fun f₀ => forall x : El A, (B x).2 (f₀ x)).
-
-Notation "A →ᶠ B" := (Prodᶠ A (fun _ => B)) (at level 99, right associativity, B at level 200).
-Notation "'Πᶠ'  x .. y , P" := (Prodᶠ _ (fun x => .. (Prodᶠ _ (fun y => P)) ..))
-  (at level 200, x binder, y binder, right associativity).
-
-Definition Lamᶠ {A : El Typeᶠ} {B : El A -> El Typeᶠ} (f : forall x : El A, El (B x)) : El (Prodᶠ A B).
-Proof.
-unshelve refine (_ ; _).
-+ refine (fun x => (f x).1).
-+ refine (fun x => (f x).2).
-Defined.
-
-Notation "'λᶠ'  x .. y , t" := (Lamᶠ (fun x => .. (Lamᶠ (fun y => t)) ..))
-  (at level 200, x binder, y binder, right associativity).
-
-Definition Appᶠ {A B} (f : El (Prodᶠ A B)) (x : El A) : El (B x).
-Proof.
-unshelve refine (_ ; _).
-+ refine (f.1 x).
-+ refine (f.2 x).
-Defined.
-
-Notation "t · u" := (Appᶠ t u) (at level 65, left associativity).
-
-
-Definition sigmaᵀ (A : El Typeᶠ) (P : El (A →ᶠ Typeᶠ)) : Type :=
-  sigma (El A) (fun x => El (P · x)).
-
-Definition existᵀ (A : El Typeᶠ) (P : El (A →ᶠ Typeᶠ))
-           (x : El A) (y : El (P · x)) : sigmaᵀ A P
-  := mk_sig x y.
-
-Inductive sigmaᴿ (A : El Typeᶠ) (P : El (A →ᶠ Typeᶠ)) : sigmaᵀ A P -> Type :=
-| existᴿ : forall (x : El A) (y : El (P · x)), sigmaᴿ A P (existᵀ A P x y).
-
-Definition sigmaᶠ : El (Πᶠ (A : El Typeᶠ) (P : El (A →ᶠ Typeᶠ)), Typeᶠ).
-Proof.
-refine (λᶠ A P, _).
-unshelve refine (mkTYPE _ (sigmaᴿ A P)).
-Defined.
-
-Definition existᶠ : El (Πᶠ (A : El Typeᶠ) (P : El (A →ᶠ Typeᶠ)) (x : El A) (y : El (P · x)),
-  sigmaᶠ · A · P).
-Proof.
-refine (λᶠ A P x y, _).
-refine (mk_sig (existᵀ A P x y) (existᴿ A P x y)).
-Defined.
-
-
-Implement Existing sigma.
-exact sigmaᶠ.
-Defined.
-
-Implement Existing mk_sig.
-exact existᶠ.
-Defined.
-
-
-Inductive eq2 (A : El Typeᶠ) (x : El A) :
-  forall (y : El A), eq (π1 x) (π1 y) -> Prop :=
-| refl2 : eq2 A x x eq_refl.
-
-
-Definition eqᶠ : El (Πᶠ (A : El Typeᶠ), A →ᶠ A →ᶠ Typeᶠ).
-Proof.
-refine (λᶠ A x y, _).
-unshelve refine (mkTYPE _ _).
-+ refine (eq x.1 y.1).
-+ refine (eq2 A x y).
-Defined.
-
-Implement Existing eq.
-unshelve econstructor.
-exact (fun A x y => π1 x = π1 y).
-exact eq2.
-Defined.
-
-
-Definition reflᶠ : El (Πᶠ (A : El Typeᶠ) (x : El A), eqᶠ · A · x · x).
-Proof.
-refine (λᶠ A x, _).
-unshelve refine (_; refl2 A x).
-Defined.
-
-
-
-Notation " A × B " := (sigma A (fun _ => B)) (at level 30) : type_scope.
-
-
-Definition equiv (A B : Type) :=
-  exists (f : A -> B) (g : B -> A), (forall x, g (f x) = x) × (forall y, f (g y) = y).
-Translate equiv.
-
-Implement Existing False.
-exact (False; fun _ => False).
-Defined.
-
-Definition not A := A -> False.
-Translate not.
-
-(* Definition hasTwoElements A *)
-(*   := exists x y, @eq A x y -> False. *)
-(* Translate hasTwoElements. *)
-
-Definition HasTwoElFstComponentᶠ : El (Typeᶠ →ᶠ Typeᶠ) :=
-  λᶠ (T : El Typeᶠ), mkTYPE (exists (x y : T.1), x = y -> False) (fun _ => unit).
-
-Implement notUnivalence :
-  exists A B, (equiv A B) × exists P, P A × not (P B).
-Proof.
-simple refine (existᶠ · _ · _ · _ · _).
-exact (bool:Type; fun _=> unit:Type).
-simple refine (existᶠ · _ · _ · _ · _).
-exact (unit:Type; fun _ => bool:Type).
-simple refine (existᶠ · _ · _ · _ · _).
-- simple refine (existᶠ · _ · _ · _ · _).
-  exists π2. exact π1.
-  simple refine (existᶠ · _ · _ · _ · _).
-  exists π2. exact π1.
-  simple refine (existᶠ · _ · _ · _ · _);
-    cbn; unshelve econstructor; reflexivity.
-- simple refine (existᶠ · _ · _ · _ · _).
-  exact HasTwoElFstComponentᶠ.
-  simple refine (existᶠ · _ · _ · _ · _).
-  + cbn. refine (_; tt). exists true. exists false.
-    discriminate 1.
-  + refine (λᶠ p, _). cbn in p.
-    destruct p as [p _].
-    destruct p as [[] [[] p]].
-    contradiction p. reflexivity.
-Defined.
-
-
-
-
-
-  
-(* ** Some check of the translation on other types. *** *)
-
 Implement f : forall (f : Type -> Type), f Type.
 Abort.
 
@@ -378,5 +149,6 @@ Abort.
 Implement wqd : forall (A : Type) (B : A -> Prop), forall x, B x.
 Abort.
 
-(* Implement foo : forall (A : Type) (a : A) (p : a = a), p = eq_refl a. *)
-(* Abort. *)
+Implement foo : forall (A : Type) (a : A) (p : a = a), p = eq_refl a.
+Abort.
+
