theories/extract_trad.v
@@ -4,7 +4,7 @@
     should use these same directives for consistency.
 *)
 
-Require Import Template.translation_utils Template.tsl_param Template.tsl_fun.
+Require Import Template.translation_utils Template.tsl_param Template.tsl_fun Template.tsl_p.
 
 Require Import ExtrOcamlBasic.
 Require Import ExtrOcamlString.
@@ -14,3 +14,4 @@ Extraction Blacklist Ast String List Nat Typing.
 Extraction Library translation_utils.
 Extraction Library tsl_param.
 Extraction Library tsl_fun.
+Extraction Library tsl_p.
